lean/nat/lemmas.lean
@@ -102,99 +102,13 @@ lemma div_pow_mono {x n i : ℕ} (h: x < 2^n) : x / 2^i < 2^n :=
       x / 2^i ≤ x   : nat.div_le_self x (2^i)
           ... < 2^n : h
 
-lemma sshr_in_range_n_le_i {n i x : ℕ} (hx: x < 2^n) (hni: n ≤ i) : 2^n - 2^(n-i) + x/2^i < 2^n :=
-  begin
-    simp [nat.sub_eq_zero_of_le hni],
-    rw div_eq_of_lt,
-    { simp,
-      apply sub_lt_of_pos_le,
-      { dec_trivial_tac },
-      { apply pos_pow_of_pos,
-        dec_trivial_tac,
-      },
-    },
-    { apply nat.lt_of_lt_of_le,
-      { exact hx },
-      { apply pow_le_pow_of_le_right,
-        dec_trivial_tac,
-        exact hni,
-      },
-    },
-  end
-
-lemma sshr_in_range_i_lt_n_2 {n i x : ℕ} (hx: x < 2^n) (hni: i < n) : 2^n - 2^(n-i) + x/2^i < 2^n :=
-  begin
-    cases i, -- This is slightly annoying, but we need to prove
-             -- the i = 0 case separately so we can use i > 0
-             -- for sub_lt_of_pos_le as the argument to
-             -- pow_lt_pow_of_lt_right in the other case.
-    case nat.zero
-    { simp, rw nat.sub_self (2^n), simp, exact hx },
-      case nat.succ
-      { have i_lt_n : succ i ≤ n,
-        { apply le_of_lt hni },
-        have : x/2^succ i < 2^(n-succ i),
-        { apply div_lt_of_lt_mul,
-        apply pos_pow_of_pos,
-        dec_trivial_tac,
-        rw [pow_mul, add_sub_of_le],
-        apply hx,
-        apply i_lt_n
-      },
-      apply sub_add_lt_self (2^n) (2^(n-succ i)) (x/2^(succ i)) _ this,
-      apply pow_lt_pow_of_lt_right (lt_succ_self _)
-                                   (sub_lt_of_pos_le _ _ (nat.zero_lt_succ i) i_lt_n)
-    }
-  end
-
-lemma sshr_in_range_i_lt_n_i_pos {n i x : ℕ} (hx: x < 2^n) (hni: i < n) (hipos: i > 0)
-: 2^n - 2^(n-i) + x/2^i < 2^n :=
-  begin
-  { have i_le_n : i ≤ n, { apply le_of_lt hni },
-    have x_div_lt : x/2^i < 2^(n-i),
-    { apply div_lt_of_lt_mul,
-      apply pos_pow_of_pos,
-      dec_trivial_tac,
-      rw [pow_mul, add_sub_of_le],
-      apply hx,
-      apply i_le_n
-    },
-    apply sub_add_lt_self (2^n) (2^(n-i)) (x/2^i) _ x_div_lt,
-    apply pow_lt_pow_of_lt_right,
-    { dec_trivial_tac },
-    { apply sub_lt_of_pos_le i n hipos,
-      apply le_of_lt hni
-    },
-  }
-  end
-
-lemma sshr_in_range_i_lt_n {n i x : ℕ} (hx: x < 2^n) (hni: i < n) : 2^n - 2^(n-i) + x/2^i < 2^n :=
-  begin
-    -- We case on i because when i is positive, the cruxt of the
-    -- proof is applying pow_lt_pow_of_lt_right (which requires i > 0)
-    -- (see sshr_in_range_i_lt_n_i_pos).
-    --
-    -- The case when i = 0 basically follows from hx once you
-    -- simplify.
-    by_cases i_cmp_zero : i > 0,
-    { apply sshr_in_range_i_lt_n_i_pos hx hni i_cmp_zero },
-    { have i_zero : i = 0,
-      { apply eq_zero_of_le_zero,
-        apply le_of_not_gt i_cmp_zero,
-      },
-      simp [i_zero, nat.sub_self (2^n)],
-      exact hx
-    },
-  end
-
-lemma sshr_in_range {n i x : ℕ} (h: x < 2^n) : 2^n - 2^(n-i) + x/2^i < 2^n :=
-  begin
-    by_cases this : n ≤ i,
-    { apply sshr_in_range_n_le_i h this },
-    { apply sshr_in_range_i_lt_n h (lt_of_not_ge this) },
-  end
-
 lemma pow_mod_superfluous {x n m : ℕ} (H : x < 2 ^ n) (Hm: m ≤ n): (x / 2 ^ m % 2 ^ (n - m)) = x / 2 ^ m :=
 begin
   apply mod_eq_of_lt, apply (div_pow_mono' H Hm)
 end
+
+lemma nat_sub_le_self (a b : ℕ) (h: a ≥ b) : a - b ≤ a :=
+  begin
+    apply le_of_lt_succ,
+    apply sub_lt_succ
+  end
